wip; an abstract type of base_key in bijection with BinTree.key

steel/Zeta.Steel.KeyUtils.fst
@@ -1,22 +1,24 @@
 module Zeta.Steel.KeyUtils
 open FStar.Ghost
-open Zeta.Steel.ApplicationTypes
 module U8 = FStar.UInt8
 module U16 = FStar.UInt16
 module U32 = FStar.UInt32
 module U64 = FStar.UInt64
-open Zeta.Steel.FormatsManual
-module T = Zeta.Steel.FormatsManual
 module C = FStar.Int.Cast
 
-let root_base_key: T.base_key =
-  let open T in
+let significant_digits_t =
+  significant_digits: U16.t { U16.v significant_digits <= 256 }
+
+type raw_key = {
+  k: u256;
+  significant_digits : significant_digits_t;
+}
+
+let root_raw_key: raw_key =
   {
     k = { v3 = U64.zero; v2 = U64.zero ; v1 = U64.zero ; v0 = U64.zero };
     significant_digits = U16.zero;
   }
-
-let root_key: T.key = InternalKey root_base_key
 
 let bit_offset_in_word (i:U16.t { U16.v i < 256 })
   : U32.t & U32.t
@@ -36,9 +38,9 @@ let truncate_word (k:U64.t) (index:U32.t { U32.v index < 64 })
          let mask = U64.shift_right 0xffffffffffffffffuL shift_index in
          U64.logand k mask
 
-let truncate_key (k:T.base_key)
-                 (w:U16.t { U16.v w <= U16.v k.T.significant_digits })
-  : T.base_key
+let truncate_key (k:raw_key)
+                 (w:U16.t { U16.v w <= U16.v k.significant_digits })
+  : raw_key
   = let open U16 in
     if w = k.significant_digits then k
     else (
@@ -56,18 +58,11 @@ let truncate_key (k:T.base_key)
       { k = kk'; significant_digits = w }
     )
 
-let is_proper_descendent (k0 k1:T.base_key)
+let is_proper_descendent' (k0 k1:raw_key)
   : bool
   = let open FStar.UInt16 in
-    k0.T.significant_digits >^ k1.T.significant_digits &&
-    truncate_key k0 k1.T.significant_digits = k1
-
-let is_proper_descendent_key_type (k0 k1:T.internal_key)
-  : Lemma
-    (requires is_proper_descendent k0 k1)
-    (ensures  not (T.is_internal_key_for_data k1))
-    [SMTPat (is_proper_descendent k0 k1)]
-  = ()
+    k0.significant_digits >^ k1.significant_digits &&
+    truncate_key k0 k1.significant_digits = k1
 
 let nth_63_mod2 (x:U64.t)
   : Lemma (UInt.nth (U64.v x) 63 == (U64.v x % 2 = 1))
@@ -96,21 +91,21 @@ let ith_bit_64_extensional (x y:U64.t)
     );
     UInt.nth_lemma #64 (U64.v x) (U64.v y)
 
-let ith_bit (k0:T.base_key) (i:U16.t { U16.v i < 256 })
+let ith_bit (k0:raw_key) (i:U16.t { U16.v i < 256 })
   : bool
   = let open U16 in
-    let kk = k0.T.k in
+    let kk = k0.k in
     let word, bit = bit_offset_in_word i in
     if word = 0ul
-    then ith_bit_64 kk.T.v0 bit
+    then ith_bit_64 kk.v0 bit
     else if word = 1ul
-    then ith_bit_64 kk.T.v1 bit
+    then ith_bit_64 kk.v1 bit
     else if word = 2ul
-    then ith_bit_64 kk.T.v2 bit
-    else ith_bit_64 kk.T.v3 bit
+    then ith_bit_64 kk.v2 bit
+    else ith_bit_64 kk.v3 bit
 
 #push-options "--fuel 0 --ifuel 0"
-let ith_bit_extensional (x y:T.base_key)
+let ith_bit_extensional (x y:raw_key)
   : Lemma
     (requires
       x.significant_digits == y.significant_digits /\
@@ -142,10 +137,10 @@ let ith_bit_extensional (x y:T.base_key)
     ith_bit_64_extensional x.k.v3 y.k.v3
 #pop-options
 
-let set_ith_bit (k0:T.base_key) (i:U16.t { U16.v i < 256 })
-  : GTot T.base_key
+let set_ith_bit (k0:raw_key) (i:U16.t { U16.v i < 256 })
+  : GTot raw_key
   = let open U16 in
-    let kk = k0.T.k in
+    let kk = k0.k in
     let word, bit = bit_offset_in_word i in
     let mask = U64.shift_left 1uL bit in
     let kk' =
@@ -166,10 +161,10 @@ let clear_ith_bit_64 (k:U64.t) (i:U32.t { U32.v i < 64 })
     let v' = Seq.upd v index false in
     U64.uint_to_t (UInt.from_vec #64 v')
 
-let clear_ith_bit (k0:T.base_key) (i:U16.t { U16.v i < 256 })
-  : GTot T.base_key
+let clear_ith_bit (k0:raw_key) (i:U16.t { U16.v i < 256 })
+  : GTot raw_key
   = let open U16 in
-    let kk = k0.T.k in
+    let kk = k0.k in
     let word, bit = bit_offset_in_word i in
     let kk' =
       if word = 0ul
@@ -184,7 +179,7 @@ let clear_ith_bit (k0:T.base_key) (i:U16.t { U16.v i < 256 })
 
 #push-options "--fuel 0 --ifuel 0"
 
-let set_get_ith_bit_core (k:T.base_key) (i:U16.t { U16.v i < 256 })
+let set_get_ith_bit_core (k:raw_key) (i:U16.t { U16.v i < 256 })
   : Lemma ((ith_bit (set_ith_bit k i) i == true))
   = let open U16 in
     let k' = set_ith_bit k i in
@@ -218,7 +213,7 @@ let set_get_ith_bit_core (k:T.base_key) (i:U16.t { U16.v i < 256 })
         true;
       }
 
-let set_ith_bit_modifies (k:T.base_key)
+let set_ith_bit_modifies (k:raw_key)
                          (i:U16.t { U16.v i < 256 })
                          (j:U16.t { U16.v j <> U16.v i /\ U16.v j < 256 })
   : Lemma ((ith_bit (set_ith_bit k i) j == ith_bit k j))
@@ -284,11 +279,11 @@ let clear_ith_bit_64_spec (k:U64.t) (i:U32.t { U32.v i < 64 })
   = FStar.Classical.forall_intro (ith_bit_64_nth (clear_ith_bit_64 k i));
     FStar.Classical.forall_intro (ith_bit_64_nth k)
 
-let clear_get_ith_bit_core (k:T.base_key) (i:U16.t { U16.v i < 256 })
+let clear_get_ith_bit_core (k:raw_key) (i:U16.t { U16.v i < 256 })
   : Lemma (ith_bit (clear_ith_bit k i) i == false)
   = FStar.Classical.forall_intro_2 clear_ith_bit_64_spec
 
-let clear_ith_bit_modifies (k:T.base_key)
+let clear_ith_bit_modifies (k:raw_key)
                          (i:U16.t { U16.v i < 256 })
                          (j:U16.t { U16.v j <> U16.v i /\ U16.v j < 256 })
   : Lemma (ith_bit (clear_ith_bit k i) j == ith_bit k j)
@@ -296,13 +291,13 @@ let clear_ith_bit_modifies (k:T.base_key)
 
 #pop-options
 
-let set_get_ith_bit (k:T.base_key) (i:U16.t { U16.v i < 256 })
+let set_get_ith_bit (k:raw_key) (i:U16.t { U16.v i < 256 })
   : Lemma ((ith_bit (set_ith_bit k i) i == true) /\
             (forall (j:U16.t { j <> i /\ U16.v j < 256 }). ith_bit (set_ith_bit k i) j == ith_bit k j))
   = set_get_ith_bit_core k i;
     FStar.Classical.forall_intro (set_ith_bit_modifies k i)
 
-let clear_set_ith_bit (k:T.base_key) (i:U16.t { U16.v i < 256 })
+let clear_set_ith_bit (k:raw_key) (i:U16.t { U16.v i < 256 })
   : Lemma (clear_ith_bit (set_ith_bit k i) i ==
            clear_ith_bit k i)
   = FStar.Classical.forall_intro_2 clear_get_ith_bit_core;
@@ -311,24 +306,24 @@ let clear_set_ith_bit (k:T.base_key) (i:U16.t { U16.v i < 256 })
     ith_bit_extensional (clear_ith_bit (set_ith_bit k i) i)
                         (clear_ith_bit k i)
 
-let clear_ith_bit_elim (k:T.base_key) (i:U16.t { U16.v i < 256 })
+let clear_ith_bit_elim (k:raw_key) (i:U16.t { U16.v i < 256 })
   : Lemma (requires ith_bit k i = false)
           (ensures clear_ith_bit k i == k)
   = FStar.Classical.forall_intro_2 clear_get_ith_bit_core;
     FStar.Classical.forall_intro_3 clear_ith_bit_modifies;
     ith_bit_extensional (clear_ith_bit k i) k
 
-let ith_bit_root_base_key (i:U16.t { U16.v i < 256 })
-  : Lemma (ith_bit root_base_key i == false)
+let ith_bit_root_raw_key (i:U16.t { U16.v i < 256 })
+  : Lemma (ith_bit root_raw_key i == false)
   = let open U16 in
-    let res = ith_bit root_base_key i in
-    let kk = root_base_key.k in
+    let res = ith_bit root_raw_key i in
+    let kk = root_raw_key.k in
     let word, bit = bit_offset_in_word i in
     FStar.UInt.shift_right_value_lemma #64 0 (U32.v bit);
     FStar.Math.Lemmas.small_div 0 (pow2 (U32.v bit))
 
 (* if you lift a lowered key, you get the original key, but not the other way round *)
-let rec lift_base_key (k: T.base_key)
+let rec lift_raw_key (k: raw_key)
   : GTot (k':Zeta.Key.base_key {
                Zeta.BinTree.depth k' = U16.v k.significant_digits
           })
@@ -337,18 +332,18 @@ let rec lift_base_key (k: T.base_key)
     let open Zeta.BinTree in
     if k.significant_digits = 0us then Root
     else let i = k.significant_digits -^ 1us in
-         let k' = lift_base_key ({k with significant_digits = i }) in
+         let k' = lift_raw_key ({k with significant_digits = i }) in
          if ith_bit k i
          then RightChild k'
          else LeftChild k'
 
 let rec lower_base_key' (k: Zeta.Key.base_key)
-  : GTot (k':T.base_key {
+  : GTot (k':raw_key {
                 U16.v k'.significant_digits = Zeta.BinTree.depth k
           })
   = let open Zeta.BinTree in
     match k with
-    | Root -> root_base_key
+    | Root -> root_raw_key
 
     | LeftChild k ->
       let k' = lower_base_key' k in
@@ -368,7 +363,7 @@ let rec lower_base_key_significant_digits (k: Zeta.Key.base_key)
   = let open Zeta.BinTree in
     match k with
     | Root ->
-      FStar.Classical.forall_intro ith_bit_root_base_key
+      FStar.Classical.forall_intro ith_bit_root_raw_key
 
     | LeftChild k ->
       lower_base_key_significant_digits k
@@ -378,21 +373,21 @@ let rec lower_base_key_significant_digits (k: Zeta.Key.base_key)
       let kk = lower_base_key' k in
       set_get_ith_bit kk kk.significant_digits
 
-let rec lift_base_key_irrelevant_bits (b0 b1:T.base_key)
+let rec lift_raw_key_irrelevant_bits (b0 b1:raw_key)
   : Lemma
     (requires b0.significant_digits = b1.significant_digits /\
               (forall (i:U16.t{U16.v i < U16.v b0.significant_digits}).{:pattern (has_type i U16.t)} ith_bit b0 i == ith_bit b1 i))
-    (ensures  lift_base_key b0 == lift_base_key b1)
+    (ensures  lift_raw_key b0 == lift_raw_key b1)
     (decreases U16.v b0.significant_digits)
   = if b0.significant_digits = 0us then ()
     else (
       let b0' = { b0 with significant_digits = U16.(b0.significant_digits -^ 1us) } in
       let b1' = { b1 with significant_digits = U16.(b1.significant_digits -^ 1us) } in
-      lift_base_key_irrelevant_bits b0' b1'
+      lift_raw_key_irrelevant_bits b0' b1'
     )
 
 let rec lift_lower_id (k:Zeta.Key.base_key)
-  : Lemma (lift_base_key (lower_base_key' k) == k)
+  : Lemma (lift_raw_key (lower_base_key' k) == k)
   = let open U16 in
     let open Zeta.BinTree in
     match k with
@@ -404,58 +399,59 @@ let rec lift_lower_id (k:Zeta.Key.base_key)
       lift_lower_id k';
       lower_base_key_significant_digits k';
       let k0' = lower_base_key' k' in
-      assert (lift_base_key k0' == k');
+      assert (lift_raw_key k0' == k');
       set_get_ith_bit k0' k0'.significant_digits;
       let k0 = lower_base_key' k in
       assert (ith_bit k0 k0'.significant_digits);
       assert (k0.significant_digits <> 0us);
       calc (==) {
-          lift_base_key k0;
+          lift_raw_key k0;
       (==) {}
-          RightChild (lift_base_key ({k0 with significant_digits = k0.significant_digits -^ 1us }));
-      (==) { lift_base_key_irrelevant_bits k0' ({k0 with significant_digits = k0.significant_digits -^ 1us }) }
-          RightChild (lift_base_key k0');
+          RightChild (lift_raw_key ({k0 with significant_digits = k0.significant_digits -^ 1us }));
+      (==) { lift_raw_key_irrelevant_bits k0' ({k0 with significant_digits = k0.significant_digits -^ 1us }) }
+          RightChild (lift_raw_key k0');
       }
 
-let lower_base_key (k: Zeta.Key.base_key)
-  : GTot (k':T.base_key {
-                lift_base_key k' = k
+let lower_base_key_raw (k: Zeta.Key.base_key)
+  : GTot (k':raw_key {
+                lift_raw_key k' = k
           })
   = lift_lower_id k;
     lower_base_key' k
-let desc_dir (k0:T.base_key) (k1:T.base_key { k0 `is_proper_descendent` k1 })
+
+let desc_dir_raw (k0:raw_key) (k1:raw_key { k0 `is_proper_descendent'` k1 })
   : bool
   = let open U16 in
-    not (ith_bit k0 k1.T.significant_digits)
+    not (ith_bit k0 k1.significant_digits)
 
-let parent (k:T.base_key { k.significant_digits <> 0us })
-  : GTot T.base_key
+let parent (k:raw_key { k.significant_digits <> 0us })
+  : GTot raw_key
   = let i = U16.(k.significant_digits -^ 1us) in
     if ith_bit k i
     then { clear_ith_bit k i with significant_digits = i }
     else { k with significant_digits = i }
 
 #push-options "--query_stats --fuel 1 --ifuel 0 --z3rlimit_factor 10"
-let is_parent_related (k:T.base_key { k.significant_digits <> 0us })
+let is_parent_related (k:raw_key { k.significant_digits <> 0us })
                       (ik:Zeta.Key.base_key)
   : Lemma
-    (requires k == lower_base_key ik)
-    (ensures parent k == lower_base_key (Zeta.BinTree.parent ik))
+    (requires k == lower_base_key_raw ik)
+    (ensures parent k == lower_base_key_raw (Zeta.BinTree.parent ik))
   = let open U16 in
     match ik with
     | Zeta.BinTree.LeftChild ik' ->
-      let sk' = lower_base_key ik' in
+      let sk' = lower_base_key_raw ik' in
       calc (==) {
-        lower_base_key (Zeta.BinTree.parent ik);
+        lower_base_key_raw (Zeta.BinTree.parent ik);
        (==) {}
-        lower_base_key ik';
+        lower_base_key_raw ik';
        (==) {}
-        { lower_base_key ik with significant_digits = sk'.significant_digits };
+        { lower_base_key_raw ik with significant_digits = sk'.significant_digits };
        (==) { }
         parent k;
       }
     | Zeta.BinTree.RightChild ik' ->
-      let sk' = lower_base_key ik' in
+      let sk' = lower_base_key_raw ik' in
       assert (Zeta.BinTree.parent ik == ik');
       calc (==) {
         lower_base_key' (Zeta.BinTree.parent ik);
@@ -476,21 +472,21 @@ let is_parent_related (k:T.base_key { k.significant_digits <> 0us })
         parent k;
       }
 
-let rec is_desc (k0 k1:T.base_key)
+let rec is_desc_raw (k0 k1:raw_key)
   : GTot bool (decreases (U16.v (k0.significant_digits)))
   = if k0 = k1
     then true
     else if k0.significant_digits = 0us
     then false
-    else is_desc (parent k0) k1
+    else is_desc_raw (parent k0) k1
 
-let rec is_desc_related (k0 k1:T.base_key) (ik0 ik1:Zeta.Key.base_key)
+let rec is_desc_raw_related (k0 k1:raw_key) (ik0 ik1:Zeta.Key.base_key)
   : Lemma
     (requires
-      k0 == lower_base_key ik0 /\
-      k1 == lower_base_key ik1)
+      k0 == lower_base_key_raw ik0 /\
+      k1 == lower_base_key_raw ik1)
     (ensures
-      is_desc k0 k1 == Zeta.BinTree.is_desc_aux ik0 ik1)
+      is_desc_raw k0 k1 == Zeta.BinTree.is_desc_aux ik0 ik1)
     (decreases (U16.v k0.significant_digits))
   = if k0 = k1 then ()
     else if k0.significant_digits = 0us then (
@@ -498,17 +494,17 @@ let rec is_desc_related (k0 k1:T.base_key) (ik0 ik1:Zeta.Key.base_key)
     )
     else (
       is_parent_related k0 ik0;
-      is_desc_related (parent k0) k1 (Zeta.BinTree.parent ik0) ik1
+      is_desc_raw_related (parent k0) k1 (Zeta.BinTree.parent ik0) ik1
     )
 
-let rec truncate_key_spec (k:T.base_key)
+let rec truncate_key_spec (k:raw_key)
                           (w:U16.t{U16.v w <= U16.v k.significant_digits })
-  : GTot (k':T.base_key {k'.significant_digits == w})
+  : GTot (k':raw_key {k'.significant_digits == w})
          (decreases (U16.v k.significant_digits))
   = if k.significant_digits = w then k
     else truncate_key_spec (parent k) w
 
-let rec truncate_key_spec_ith_bit (k:T.base_key)
+let rec truncate_key_spec_ith_bit (k:raw_key)
                                   (w:U16.t{U16.v w <= U16.v k.significant_digits })
   : Lemma
     (ensures (
@@ -572,7 +568,7 @@ let truncate_word_ith_bit (k:U64.t)
 #pop-options
 
 #push-options "--fuel 0 --ifuel 1"
-let truncate_key_ith_bit (k:T.base_key)
+let truncate_key_ith_bit (k:raw_key)
                          (w:U16.t{U16.v w <= U16.v k.significant_digits })
   : Lemma
     (ensures (
@@ -618,58 +614,58 @@ let truncate_key_ith_bit (k:T.base_key)
     )
 #pop-options
 
-let good_key (k:T.base_key)
+let good_raw_key (k:raw_key)
   = forall (i:U16.t { U16.v i < 256 && U16.v i >= U16.v k.significant_digits }). ith_bit k i = false
 
-let truncate_key_correct (k:T.base_key) (w:U16.t { U16.v w <= U16.v k.significant_digits })
+let truncate_key_correct (k:raw_key) (w:U16.t { U16.v w <= U16.v k.significant_digits })
   : Lemma
-    (requires good_key k)
+    (requires good_raw_key k)
     (ensures truncate_key k w == truncate_key_spec k w)
   = truncate_key_ith_bit k w;
     truncate_key_spec_ith_bit k w;
     ith_bit_extensional (truncate_key k w) (truncate_key_spec k w)
 
-let rec is_desc_significant_digits (k0 k1:T.base_key)
+let rec is_desc_significant_digits (k0 k1:raw_key)
   : Lemma
-    (requires is_desc k0 k1)
+    (requires is_desc_raw k0 k1)
     (ensures (U16.v k0.significant_digits >= U16.v k1.significant_digits /\
              (U16.v k0.significant_digits = U16.v k1.significant_digits  ==> k0 == k1)))
     (decreases U16.v k0.significant_digits)
   = if k0 = k1 then ()
     else is_desc_significant_digits (parent k0) k1
 
-let rec is_desc_truncate_key_spec (k0 k1:T.base_key)
+let rec is_desc_truncate_key_spec (k0 k1:raw_key)
   : Lemma
     (requires U16.v k0.significant_digits >= U16.v k1.significant_digits)
-    (ensures is_desc k0 k1 == (truncate_key_spec k0 k1.significant_digits = k1))
+    (ensures is_desc_raw k0 k1 == (truncate_key_spec k0 k1.significant_digits = k1))
     (decreases (U16.v k0.significant_digits))
   = if k0 = k1 then ()
     else if k0.significant_digits = k1.significant_digits
     then (
       assert (truncate_key_spec k0 k1.significant_digits == k0);
-      if is_desc k0 k1
+      if is_desc_raw k0 k1
       then is_desc_significant_digits k0 k1
     )
     else is_desc_truncate_key_spec (parent k0) k1
 
-let truncate_is_desc (k0 k1:T.base_key)
+let truncate_is_desc (k0 k1:raw_key)
   : Lemma
     (requires
-      good_key k0 /\
+      good_raw_key k0 /\
       U16.v k0.significant_digits >= U16.v k1.significant_digits)
-    (ensures is_desc k0 k1 ==  (truncate_key k0 k1.T.significant_digits = k1))
+    (ensures is_desc_raw k0 k1 ==  (truncate_key k0 k1.significant_digits = k1))
   = truncate_key_correct k0 k1.significant_digits;
     is_desc_truncate_key_spec k0 k1
 
-let is_proper_descendent_correct (k0 k1:T.base_key)
+let is_proper_descendent_raw_correct (k0 k1:raw_key)
   : Lemma
-    (requires good_key k0)
+    (requires good_raw_key k0)
     (ensures
-      is_proper_descendent k0 k1 == (k0 <> k1 && is_desc k0 k1))
+      is_proper_descendent' k0 k1 == (k0 <> k1 && is_desc_raw k0 k1))
   = if U16.v k0.significant_digits < U16.v k1.significant_digits
     then (
-      assert (not (is_proper_descendent k0 k1));
-      if is_desc k0 k1
+      assert (not (is_proper_descendent' k0 k1));
+      if is_desc_raw k0 k1
       then is_desc_significant_digits k0 k1
     )
     else truncate_is_desc k0 k1
@@ -677,7 +673,7 @@ let is_proper_descendent_correct (k0 k1:T.base_key)
 #push-options "--fuel 1 --ifuel 1"
 let rec lowered_keys_are_good (ik:Zeta.Key.base_key)
   : Lemma
-    (ensures good_key (lower_base_key' ik))
+    (ensures good_raw_key (lower_base_key' ik))
     (decreases ik)
   = let sk = lower_base_key' ik in
     match ik with
@@ -697,23 +693,23 @@ let rec lowered_keys_are_good (ik:Zeta.Key.base_key)
         FStar.Classical.forall_intro (set_ith_bit_modifies sk' sk'.significant_digits)
       )
 
-let related_proper_descendent (sk0 sk1: T.base_key)
-                              (ik0 ik1: Zeta.Key.base_key)
+let related_proper_descendent_raw (sk0 sk1: raw_key)
+                                  (ik0 ik1: Zeta.Key.base_key)
   : Lemma
     (requires
-      sk0 == lower_base_key ik0 /\
-      sk1 == lower_base_key ik1)
+      sk0 == lower_base_key_raw ik0 /\
+      sk1 == lower_base_key_raw ik1)
     (ensures
-      is_proper_descendent sk0 sk1 = Zeta.BinTree.is_proper_desc ik0 ik1)
+      is_proper_descendent' sk0 sk1 = Zeta.BinTree.is_proper_desc ik0 ik1)
   = lowered_keys_are_good ik0;
-    is_proper_descendent_correct sk0 sk1;
+    is_proper_descendent_raw_correct sk0 sk1;
     Zeta.BinTree.is_desc_eq ik0 ik1;
-    is_desc_related sk0 sk1 ik0 ik1
+    is_desc_raw_related sk0 sk1 ik0 ik1
 
-let truncate_key_extension (k:T.base_key)
+let truncate_key_extension (k:raw_key)
                            (w:U16.t { U16.(w <^ k.significant_digits) })
   : Lemma
-    (requires good_key k)
+    (requires good_raw_key k)
     (ensures (
       let k0 = truncate_key_spec k w in
       let k' = truncate_key_spec k U16.(w +^ 1us) in
@@ -752,26 +748,26 @@ let truncate_key_extension (k:T.base_key)
     )
 
 module B = Zeta.BinTree
-let related_desc_dir (sk0 sk1: T.base_key) (ik0 ik1: Zeta.Key.base_key)
+let related_desc_dir_raw (sk0 sk1: raw_key) (ik0 ik1: Zeta.Key.base_key)
   : Lemma
     (requires
-      sk0 == lower_base_key ik0 /\
-      sk1 == lower_base_key ik1 /\
-      is_proper_descendent sk0 sk1)
+      sk0 == lower_base_key_raw ik0 /\
+      sk1 == lower_base_key_raw ik1 /\
+      is_proper_descendent' sk0 sk1)
     (ensures (
-      related_proper_descendent sk0 sk1 ik0 ik1;
-      desc_dir sk0 sk1 == (Zeta.BinTree.Left? (Zeta.BinTree.desc_dir ik0 ik1))))
-  = related_proper_descendent sk0 sk1 ik0 ik1;
+      related_proper_descendent_raw sk0 sk1 ik0 ik1;
+      desc_dir_raw sk0 sk1 == (Zeta.BinTree.Left? (Zeta.BinTree.desc_dir ik0 ik1))))
+  = related_proper_descendent_raw sk0 sk1 ik0 ik1;
     lowered_keys_are_good ik0;
     lowered_keys_are_good ik1;
     let c = B.desc_dir ik0 ik1 in
-    if desc_dir sk0 sk1
+    if desc_dir_raw sk0 sk1
     then (
       assert (not (ith_bit sk0 sk1.significant_digits));
       assert (truncate_key sk0 sk1.significant_digits ==
-              lower_base_key ik1);
+              lower_base_key_raw ik1);
       assert (ith_bit
-               (lower_base_key (B.LeftChild ik1))
+               (lower_base_key_raw (B.LeftChild ik1))
                sk1.significant_digits = false);
       calc (==) {
        truncate_key sk0 U16.(sk1.significant_digits +^ 1us);
@@ -781,14 +777,14 @@ let related_desc_dir (sk0 sk1: T.base_key) (ik0 ik1: Zeta.Key.base_key)
        ( { truncate_key_spec sk0 U16.(sk1.significant_digits) with
               significant_digits = U16.(sk1.significant_digits +^ 1us) } );
       (==) { truncate_key_correct sk0 U16.(sk1.significant_digits) }
-        lower_base_key (B.LeftChild ik1);
+        lower_base_key_raw (B.LeftChild ik1);
       };
       truncate_is_desc
         sk0
-        (lower_base_key (B.LeftChild ik1));
-      assert (is_desc sk0 (lower_base_key (B.LeftChild ik1)));
-      is_desc_related sk0
-                      (lower_base_key (B.LeftChild ik1))
+        (lower_base_key_raw (B.LeftChild ik1));
+      assert (is_desc_raw sk0 (lower_base_key_raw (B.LeftChild ik1)));
+      is_desc_raw_related sk0
+                      (lower_base_key_raw (B.LeftChild ik1))
                       ik0
                       (B.LeftChild ik1);
       B.is_desc_eq ik0 (B.LeftChild ik1);
@@ -807,23 +803,23 @@ let related_desc_dir (sk0 sk1: T.base_key) (ik0 ik1: Zeta.Key.base_key)
            with
               significant_digits = U16.(sk1.significant_digits +^ 1us) } );
       (==) { truncate_key_correct sk0 sk1.significant_digits }
-        lower_base_key (B.RightChild ik1);
+        lower_base_key_raw (B.RightChild ik1);
       };
       truncate_is_desc
         sk0
-        (lower_base_key (B.RightChild ik1));
-      assert (is_desc sk0 (lower_base_key (B.RightChild ik1)));
-      is_desc_related sk0
-                      (lower_base_key (B.RightChild ik1))
+        (lower_base_key_raw (B.RightChild ik1));
+      assert (is_desc_raw sk0 (lower_base_key_raw (B.RightChild ik1)));
+      is_desc_raw_related sk0
+                      (lower_base_key_raw (B.RightChild ik1))
                       ik0
                       (B.RightChild ik1);
       B.is_desc_eq ik0 (B.RightChild ik1);
       assert (B.is_desc ik0 (B.RightChild ik1))
     )
 
-let rec lift_base_key_relevant_bits (b0 b1:T.base_key)
+let rec lift_raw_key_relevant_bits (b0 b1:raw_key)
   : Lemma
-    (requires  lift_base_key b0 == lift_base_key b1)    
+    (requires  lift_raw_key b0 == lift_raw_key b1)    
     (ensures   b0.significant_digits = b1.significant_digits /\
               (forall (i:U16.t{U16.v i < U16.v b0.significant_digits}).{:pattern (has_type i U16.t)} ith_bit b0 i == ith_bit b1 i))
     (decreases (U16.v b0.significant_digits))
@@ -832,25 +828,101 @@ let rec lift_base_key_relevant_bits (b0 b1:T.base_key)
     else if b0.significant_digits = b1.significant_digits then (
       let b0' = { b0 with significant_digits = U16.(b0.significant_digits -^ 1us) } in
       let b1' = { b1 with significant_digits = U16.(b1.significant_digits -^ 1us) } in
-      lift_base_key_relevant_bits b0' b1'
+      lift_raw_key_relevant_bits b0' b1'
     )
     else ()
 
 #push-options "--fuel 0 --ifuel 0"
-let lower_lift_id (k:base_key)
+let lower_lift_id (k:raw_key)
   : Lemma 
-    (requires good_key k)
-    (ensures lower_base_key' (lift_base_key k) == k)
-  = let hk = lift_base_key k in
-    let k' = lower_base_key hk in
-    let hk' = lift_base_key k' in
+    (requires good_raw_key k)
+    (ensures lower_base_key' (lift_raw_key k) == k)
+  = let hk = lift_raw_key k in
+    let k' = lower_base_key_raw hk in
+    let hk' = lift_raw_key k' in
     lift_lower_id hk;
     assert (hk == hk');
     lowered_keys_are_good hk;
-    assert (good_key k');
-    lift_base_key_relevant_bits k k';
+    assert (good_raw_key k');
+    lift_raw_key_relevant_bits k k';
     ith_bit_extensional k k'
 #pop-options
 
+////////////////////////////////////////////////////////////////////////////////
+// Now the main public interface on base_keys
+////////////////////////////////////////////////////////////////////////////////
    
+let base_key = r:raw_key { good_raw_key r }
+
+let is_internal_key (r:raw_key) = U16.(r.significant_digits <^ 256us)
+
+let root_base_key : internal_key =
+  FStar.Classical.forall_intro ith_bit_root_raw_key;
+  root_raw_key
+
+let is_proper_descendent (k0 k1:base_key) 
+  : bool
+  = is_proper_descendent' k0 k1
+
+let desc_dir (k0:base_key) (k1:base_key { k0 `is_proper_descendent` k1 })
+  : bool
+  = desc_dir_raw k0 k1
+
+let lift_base_key (k: base_key)
+  : GTot Zeta.Key.base_key
+  = lift_raw_key k
+
+let lower_base_key (k:Zeta.Key.base_key)
+  : GTot base_key
+  = lowered_keys_are_good k;
+    lower_base_key_raw k
   
+let lift_lower_inv (k:Zeta.Key.base_key)
+  : Lemma (lift_base_key (lower_base_key k) == k)
+  = lift_lower_id k
+  
+let lower_lift_inv (k:base_key)
+  : Lemma (lower_base_key (lift_base_key k) == k)
+  = lower_lift_id k
+  
+let is_desc (k0 k1:base_key)
+  : GTot bool
+  = is_desc_raw k0 k1
+  
+let is_desc_related (k0 k1:base_key)
+                    (ik0 ik1:Zeta.Key.base_key)
+  : Lemma
+    (requires
+      k0 == lower_base_key ik0 /\
+      k1 == lower_base_key ik1)
+    (ensures
+      is_desc k0 k1 == Zeta.BinTree.is_desc_aux ik0 ik1)
+  = is_desc_raw_related k0 k1 ik0 ik1
+  
+let is_proper_descendent_correct (k0 k1:base_key)
+  : Lemma
+    (ensures
+      is_proper_descendent k0 k1 <==> (k0 =!= k1 /\ is_desc k0 k1))
+  = is_proper_descendent_raw_correct k0 k1
+  
+let related_proper_descendent (sk0 sk1: base_key)
+                              (ik0 ik1: Zeta.Key.base_key)
+  : Lemma
+    (requires
+      sk0 == lower_base_key ik0 /\
+      sk1 == lower_base_key ik1)
+    (ensures
+      is_proper_descendent sk0 sk1 = Zeta.BinTree.is_proper_desc ik0 ik1)
+  = related_proper_descendent_raw sk0 sk1 ik0 ik1
+  
+let related_desc_dir (sk0 sk1: base_key)
+                     (ik0 ik1: Zeta.Key.base_key)
+  : Lemma
+    (requires
+      sk0 == lower_base_key ik0 /\
+      sk1 == lower_base_key ik1 /\
+      is_proper_descendent sk0 sk1)
+    (ensures (
+      related_proper_descendent sk0 sk1 ik0 ik1;
+      desc_dir sk0 sk1 == (Zeta.BinTree.Left? (Zeta.BinTree.desc_dir ik0 ik1))))
+  = related_desc_dir_raw sk0 sk1 ik0 ik1
